@prefix dcterms: <http://purl.org/dc/terms/> .
@prefix foaf: <http://xmlns.com/foaf/0.1/> .
@prefix owl: <http://www.w3.org/2002/07/owl#> .
@prefix rdf: <http://www.w3.org/1999/02/22-rdf-syntax-ns#> .
@prefix rdfa: <http://www.w3.org/ns/rdfa#> .
@prefix rdfs: <http://www.w3.org/2000/01/rdf-schema#> .
@prefix xsd: <http://www.w3.org/2001/XMLSchema#> .

rdfa:PGClass a rdfs:Class,
        owl:Class;
    dcterms:description "is the top level class of the hierarchy" .

rdfa:Pattern a rdfs:Class,
        owl:Class;
    dcterms:description "Class to identify an (RDF) resource whose properties are to be copied to another resource" .

rdfa:PrefixOrTermMapping a rdfs:Class,
        owl:Class;
    dcterms:description "is the top level class for prefix or term mappings" .

rdfa: a owl:Ontology;
    dcterms:creator <http://www.ivan-herman.net/foaf#me>;
    dcterms:date "2013-01-18";
    dcterms:description "This document describes the RDFa Vocabulary for Term and Prefix Assignment. The Vocabulary is used to modify RDFaÂ 1.1 processing behavior.";
    dcterms:publisher <http://www.w3.org/data#W3C>;
    dcterms:title "RDFa Vocabulary for Term and Prefix Assignment, and for Processor Graph Reporting";
    rdfs:isDefinedBy <http://www.w3.org/TR/rdfa-core/#s_initialcontexts>;
    owl:versionInfo "2013-03-11 07:54:23" .

rdfa:DocumentError dcterms:description "error condition; to be used when the document fails to be fully processed as a result of non-conformant host language markup";
    rdfs:subClassOf rdfa:Error .

rdfa:Info dcterms:description "is the class for all informations";
    rdfs:subClassOf rdfa:PGClass .

rdfa:PrefixRedefinition dcterms:description "warning; to be used when a prefix, either from the initial context or inherited from an ancestor node, is redefined in an element";
    rdfs:subClassOf rdfa:Warning .

rdfa:UnresolvedCURIE dcterms:description "warning; to be used when a CURIE prefix fails to be resolved";
    rdfs:subClassOf rdfa:Warning .

rdfa:UnresolvedTerm dcterms:description "warning; to be used when a Term fails to be resolved";
    rdfs:subClassOf rdfa:Warning .

rdfa:VocabReferenceError dcterms:description "warning; to be used when the value of a @vocab attribute cannot be dereferenced, hence the vocabulary expansion cannot be completed";
    rdfs:subClassOf rdfa:Warning .

rdfa:context a rdf:Property,
        owl:ObjectProperty;
    dcterms:description "provides extra context for the error, eg, http response, an XPointer/XPath information, or simply the URI that created the error";
    rdfs:domain rdfa:PGClass .

rdfa:copy a rdf:Property,
        owl:ObjectProperty;
    dcterms:description "identifies the resource (i.e., pattern) whose properties and values should be copied to replace the current triple (retaining the subject of the triple)." .

rdfa:prefix a rdf:Property,
        owl:DatatypeProperty;
    dcterms:description "defines a prefix mapping for a URI; the value is supposed to be a NMTOKEN";
    rdfs:domain rdfa:PrefixMapping .

rdfa:term a rdf:Property,
        owl:DatatypeProperty;
    dcterms:description "defines a term mapping for a URI; the value is supposed to be a NMTOKEN";
    rdfs:domain rdfa:TermMapping .

rdfa:uri a rdf:Property,
        owl:DatatypeProperty;
    dcterms:description "defines the URI for either a prefix or a term mapping; the value is supposed to be an absolute URI";
    rdfs:domain rdfa:PrefixOrTermMapping .

rdfa:usesVocabulary a rdf:Property,
        owl:ObjectProperty;
    dcterms:description """provides a relationship between the host document and a vocabulary
	defined using the @vocab facility of RDFa1.1""" .

rdfa:vocabulary a rdf:Property,
        owl:DatatypeProperty;
    dcterms:description "defines an absolute URI to be used as a default vocabulary; the value is can be any string; for documentation purposes it is advised to use the string 'true' or 'True'." .

<http://www.ivan-herman.net/foaf#me> a foaf:Person;
    rdfs:seeAlso <http://www.ivan-herman.net/foaf>;
    foaf:mbox <mailto:ivan@w3.org>;
    foaf:name "Ivan Herman";
    foaf:title "Semantic Web Activity Lead";
    foaf:workplaceHomepage <http://www.w3.org> .

rdfa:Error dcterms:description "is the class for all error conditions";
    rdfs:subClassOf rdfa:PGClass .

rdfa:PrefixMapping dcterms:description "is the class for prefix mappings";
    rdfs:subClassOf rdfa:PrefixOrTermMapping .

rdfa:TermMapping dcterms:description "is the class for term mappings";
    rdfs:subClassOf rdfa:PrefixOrTermMapping .

rdfa:Warning dcterms:description "is the class for all warnings";
    rdfs:subClassOf rdfa:PGClass .


